0th squaring part

code/ecdsap256sha2/Hacl.Impl.LowLevel.fst
@@ -659,13 +659,16 @@ let mul f r out =
 
 
 
-val sq0: f:  lbuffer uint64 (size 4) -> result: lbuffer uint64 (size 4) -> Stack uint64
-  (requires fun h -> live h result /\ live h f)
+val sq0: f:  lbuffer uint64 (size 4) -> result: lbuffer uint64 (size 4) ->
+  memory: lbuffer uint64 (size 6) -> 
+
+Stack uint64
+  (requires fun h -> live h result /\ live h f /\ live h memory)
   (ensures fun h0 c h1 -> modifies (loc result) h0 h1
   )
 
 
-let sq0 f result = 
+let sq0 f result memory = 
   push_frame();
 
     assert_norm (pow2 64 * pow2 64 = pow2 128);
@@ -688,8 +691,14 @@ let sq0 f result =
   mul64 f0 f0 o0 temp;
   
   let h = index temp (size 0) in 
+  
   mul64 f0 f1 o1 temp;
-  let l = index o1 (size 0) in     
+
+  let l = index o1 (size 0) in   
+  upd memory (size 0) l;
+  upd memory (size 1) (index temp (size 0));
+  admit();
+    
   let c1 = add_carry_u64 (u64 0) l h o1 in 
 
   let h = index temp (size 0) in 
@@ -710,12 +719,13 @@ let sq0 f result =
 
 
 
-val sq1: f1: felem -> f3: felem -> result: felem -> 
+val sq1: f1: felem -> f3: felem -> result: felem ->  memory: lbuffer uint64 (size 6) -> 
   Stack uint64 
-  (requires fun h -> live h f1 /\ live h f3 /\ live h result /\ eq_or_disjoint f3 result /\ disjoint f1 result)
+  (requires fun h -> live h f1 /\ live h f3 /\ live h result /\ eq_or_disjoint f3 result /\ disjoint f1 result /\ live h memory
+  )
   (ensures fun h0 c h1 -> modifies (loc result) h0 h1)
 
-let sq1 f_ f4 result = 
+let sq1 f_ f4 result memory = 
   push_frame();
     let result_ = create (size 4) (u64 0) in 
   let temp = create (size 1) (u64 0) in 
@@ -731,10 +741,14 @@ let sq1 f_ f4 result =
   let o3 = sub result_ (size 3) (size 1) in 
 
 
-  mul64 f0 f1 o0 temp;
+  (* mul64 f0 f1 o0 temp;  *)
 
- 
-  let h = index temp (size 0) in 
+  upd o0 (size 0) (index memory (size 0));
+  let h = index memory (size 1) in 
+  admit();
+
+
+  
   mul64 f1 f1 o1 temp;
   let l = index o1 (size 0) in     
   let c1 = add_carry_u64 (u64 0) l h o1 in 
@@ -817,6 +831,60 @@ let sq2 f_ f4 result =
 
 
 
+val sq3: f1: felem -> f3: felem -> result: felem -> 
+  Stack uint64 
+  (requires fun h -> live h f1 /\ live h f3 /\ live h result /\ eq_or_disjoint f3 result /\ disjoint f1 result)
+  (ensures fun h0 c h1 -> modifies (loc result) h0 h1)
+
+let sq3 f_ f4 result = 
+  push_frame();
+    let result_ = create (size 4) (u64 0) in 
+  let temp = create (size 1) (u64 0) in 
+
+  let f0 = index f_ (size 0) in 
+  let f1 = index f_ (size 1) in 
+  let f2 = index f_ (size 2) in 
+  let f3 = index f_ (size 3) in 
+    
+  let o0 = sub result_ (size 0) (size 1) in 
+  let o1 = sub result_ (size 1) (size 1) in 
+  let o2 = sub result_ (size 2) (size 1) in 
+  let o3 = sub result_ (size 3) (size 1) in 
+
+
+  mul64 f0 f3 o0 temp;
+
+ 
+  let h = index temp (size 0) in 
+  mul64 f1 f3 o1 temp;
+  let l = index o1 (size 0) in     
+  let c1 = add_carry_u64 (u64 0) l h o1 in 
+
+  let h = index temp (size 0) in 
+  mul64 f2 f3 o2 temp;
+  let l = index o2 (size 0) in     
+  let c2 = add_carry_u64 c1 l h o2 in
+  
+  let h = index temp (size 0) in 
+  mul64 f3 f3 o3 temp;
+  let l = index o3 (size 0) in     
+  let c3 = add_carry_u64 c2 l h o3 in
+
+  let temp0 = index temp (size 0) in 
+  
+  let c = c3 +! temp0 in 
+
+
+  let c3 = add4 result_ f4 result in 
+  admit();
+  pop_frame();  
+  c +! c3
+
+
+
+
+
+
 
 
 
@@ -831,6 +899,9 @@ val sq: f: felem -> r: felem -> out: widefelem
 let sq f r out =
   push_frame();
     let temp = create (size 8) (u64 0) in 
+
+    let memory = create (size 6) (u64 0) in 
+  
     
   let f0 = f.(0ul) in
   let f1 = f.(1ul) in
@@ -839,7 +910,7 @@ let sq f r out =
 
     let h0 = ST.get() in 
   let b0 = sub temp (size 0) (size 4) in 
-  let c0 = sq0 r b0 in 
+  let c0 = sq0 r b0 memory in 
     upd temp (size 4) c0;
 
 
@@ -848,7 +919,7 @@ let sq f r out =
     let h1 = ST.get() in 
     let bk0 = sub temp (size 0) (size 1) in 
   let b1 = sub temp (size 1) (size 4) in   
-  let c1 = sq1 r b1 b1 in 
+  let c1 = sq1 r b1 b1 memory in 
       upd temp (size 5) c1; 
     let h2 = ST.get() in
       assert(Lib.Sequence.index (as_seq h1 bk0) 0 == Lib.Sequence.index (as_seq h1 temp) 0);
@@ -866,7 +937,7 @@ let sq f r out =
 
      let bk2 = sub temp (size 0) (size 3) in 
   let b3 = sub temp (size 3) (size 4) in 
-  let c3 = mul1_add r f3 b3 b3 in 
+  let c3 = sq3 r b3 b3 in 
     upd temp (size 7) c3;
 
     assert(Lib.Sequence.index (as_seq h3 bk2) 0 == Lib.Sequence.index (as_seq h3 temp) 0);
